---
title: Law of cosines (Khan Academy)
date: 2021-09-04 00:00
category: reference/videos
summary: Notes from the Khan Academy video series on the Law of Cosines
cover: /_media/khan-academy-law-of-cosines-cover.png
---

These are notes from the Khan Academy video series on [Law of Cosines](https://www.khanacademy.org/math/precalculus/x9e81a4f98389efdf:trig/x9e81a4f98389efdf:law-of-cosines/v/law-of-cosines-example).

## Solving for a side with the law of cosines

Given a triangle with sides A, B, and C and angle AB, if you know the length of A and B and angle AB, how can you calculate C?

If the triangle is a right-angle triangle, we can solve a missing side using Pythagoras Theorem:

$C^2 = B^2 + A^2$

For any triangle, we can use the law of cosines:

$C^2 = B^2 + A^2 - 2AB \cdot \cos(\theta)$

This expression makes sense because $\cos(90Â°) = 0$ . For a right-angle triangle, you can simply ignore the $-2AB \cdot \cos(\theta)$ component.

## Solving for an angle with the law of cosines

If the angle is unknown, we can rewrite the expression as follows:

$cos(C) = \frac{a^2 + b^2 - c^2}{2ab}$

or

$C = acos(\frac{a^2 + b^2 - c^2}{2ab})$

## Proof of the law of cosines

One way to solve the problem using the law of cosines is to convert them into two right triangles.

![Law of Cosines](/_media/khan-academy-law-of-cosines.png)

Then we can calculate the side $d$ knowing CAH: Cosine =Adjacent / Hypotenuse.

$\cos(\theta)=\frac{d}{b} \Rightarrow d = b\cos(\theta)$

We know that $e$ is $e = c - b\cos(\theta)$

Can calculate side $m$ since $m$ is opposite, we can use SOH: Sine = Opposite / Hypotenuse.

$\frac{m}{b}=\sin\theta \Rightarrow m=b \sin(\theta)$

Now we can use Pythagorean formula:

 $a^2 = m^2 + e^2$
 $a^2 = (b\sin(\theta))^2 + (c-b\cos(\theta))^2$

We can then multiply it out:

$b^2sin^2 \theta + c^2 - 2cb \cos\theta + b^2\cos^2 \theta$

We can then rearrange the expression:

$b^2 sin^2 \theta + b^2 \cos^2 \theta + c^2 - 2bc \cos \theta$

Which can be rewritten as:

$b^2(\sin^2\theta + \cos^2 \theta) + c^2 -2bc \cos \theta$

Since the first part of the expression is the product of $b^2$ and the [Pythagorean identity](https://en.wikipedia.org/wiki/Pythagorean_trigonometric_identity), we can reduce it to $b^2$

$a^2 = b^2 + c^2 -2bc \cos \theta$

And that's the formula for the law of cosines!
